wip on sum_thing

lib/Sum.v
@@ -72,4 +72,152 @@ Section Sum.
     destruct a1, a2, s;
       erewrite Syntax.state_fmapSH_size; eauto.
   Qed.
+
+  Definition sum_stores
+             (s1: Syntax.store Hdr1 Hdr1_sz)
+             (s2: Syntax.store Hdr2 Hdr2_sz) : Syntax.store Hdr Hdr_sz.
+  Admitted.
+
+  Import P4automaton.
+
+  Require Import Coq.Program.Program.
+  Locate "~=".
+  Inductive embed_conf1:
+    P4automaton.configuration (Syntax.interp a1) ->
+    P4automaton.configuration (Syntax.interp sum) ->
+    Prop :=
+  | EmbedConf1Inl:
+    forall q
+      st
+      (c1: P4automaton.configuration (Syntax.interp a1))
+      (c1': P4automaton.configuration (Syntax.interp sum)),
+      conf_state c1 = inl q ->
+      conf_state c1' = inl (inl q) ->
+      conf_buf c1 ~= conf_buf c1' ->
+      sum_stores (conf_store c1) st = conf_store c1' ->
+      embed_conf1 c1 c1'
+  | EmbedConf1Inr:
+    forall q
+      st
+      (c1: P4automaton.configuration (Syntax.interp a1))
+      (c1': P4automaton.configuration (Syntax.interp sum)),
+      conf_state c1 = inr q ->
+      conf_state c1' = inr q ->
+      conf_buf c1 ~= conf_buf c1' ->
+      sum_stores (conf_store c1) st = conf_store c1' ->
+      embed_conf1 c1 c1'.
+
+  Inductive embed_conf2:
+    P4automaton.configuration (Syntax.interp a2) ->
+    P4automaton.configuration (Syntax.interp sum) ->
+    Prop :=
+  | EmbedConf2Inl:
+    forall q
+      st
+      (c2: P4automaton.configuration (Syntax.interp a2))
+      (c2': P4automaton.configuration (Syntax.interp sum)),
+      conf_state c2 = inl q ->
+      conf_state c2' = inl (inr q) ->
+      conf_buf c2 ~= conf_buf c2' ->
+      sum_stores st (conf_store c2) = conf_store c2' ->
+      embed_conf2 c2 c2'
+  | EmbedConf2Inr:
+    forall q
+      st
+      (c2: P4automaton.configuration (Syntax.interp a2))
+      (c2': P4automaton.configuration (Syntax.interp sum)),
+      conf_state c2 = inr q ->
+      conf_state c2' = inr q ->
+      conf_buf c2 ~= conf_buf c2' ->
+      sum_stores st (conf_store c2) = conf_store c2' ->
+      embed_conf2 c2 c2'.
+
+  Inductive split_bisim (R: P4automaton.configuration (Syntax.interp sum) ->
+                            P4automaton.configuration (Syntax.interp sum) ->
+                            Prop)
+    : P4automaton.configuration (Syntax.interp a1) ->
+      P4automaton.configuration (Syntax.interp a2) ->
+      Prop :=
+  | MkBisim: forall c1 c2 c1' c2',
+      embed_conf1 c1 c1' ->
+      embed_conf2 c2 c2' ->
+      R c1' c2' ->
+      split_bisim R c1 c2.
+
+  Lemma embed_accepting1:
+    forall c1 c1',
+      embed_conf1 c1 c1' ->
+      accepting c1 <-> accepting c1'.
+  Proof.
+    unfold accepting.
+    destruct c1, c1'.
+    split; intros.
+    - inversion H; subst; simpl in *; congruence.
+    - inversion H; subst; simpl in *; congruence.
+  Qed.
+
+  Lemma embed_accepting2:
+    forall c2 c2',
+      embed_conf2 c2 c2' ->
+      accepting c2 <-> accepting c2'.
+  Proof.
+    unfold accepting.
+    destruct c2, c2'.
+    split; intros.
+    - inversion H; subst; simpl in *; congruence.
+    - inversion H; subst; simpl in *; congruence.
+  Qed.
+  
+  Require Leapfrog.Bisimulations.Semantic.
+  Lemma split_is_bisim:
+    forall R,
+      Semantic.bisimulation R ->
+      Semantic.bisimulation (split_bisim R).
+  Proof.
+    unfold Semantic.bisimulation.
+    intros.
+    split.
+    - inversion H0; subst.
+      apply H in H3.
+      destruct H3.
+      erewrite embed_accepting1 by eauto.
+      erewrite embed_accepting2 by eauto.
+      auto.
+    - admit.
+  Admitted.
+
+  Lemma sum_thing:
+    forall (q1: St1) (q2: St2),
+      P4automaton.lang_equiv_state
+        (a1 := Syntax.interp sum)
+        (a2 := Syntax.interp sum)
+        (inl q1)
+        (inr q2) ->
+      P4automaton.lang_equiv_state
+        (a1 := Syntax.interp a1)
+        (a2 := Syntax.interp a2)
+        q1
+        q2.
+  Proof.
+    unfold P4automaton.lang_equiv_state.
+    intros.
+    apply Bisimulations.Semantic.bisimilar_iff_lang_equiv.
+    setoid_rewrite Bisimulations.Semantic.bisimilar_iff_lang_equiv in H.
+    unfold Semantic.bisimilar.
+    simpl in s1, s2.
+    pose (sum_stores s1 s2) as s0.
+    specialize (H s0 s0).
+    destruct H as [R [Hbisim Hrel]].
+    exists (split_bisim R).
+    split.
+    - auto using split_is_bisim.
+    - econstructor; eauto.
+      + econstructor; simpl; eauto.
+        unfold s0.
+        reflexivity.
+      + econstructor; simpl; eauto.
+        unfold s0.
+        reflexivity.
+  Qed.
+  
 End Sum.
